big refactoring (brand_new into several files)

coq/pttdom.v
@@ -1,673 +1,271 @@
-Require Import Setoid CMorphisms.
+Require Import Setoid Morphisms.
 From mathcomp Require Import all_ssreflect.
-Require Import edone finite_quotient preliminaries bij equiv multigraph_new liso.
+Require Import edone preliminaries.
+Require Export structures.
 
 Set Implicit Arguments.
 Unset Strict Implicit.
 Unset Printing Implicit Defensive.
 Set Bullet Behavior "Strict Subproofs". 
 
-
-(* 
-   strategies:
-
-   A
-    1. 2pdom + TaT=T    (with rule G+· --> G)
-    2. 2pdom by conservativity
-    3. 2p by normalisation and reduction to 2pdom (for nfs u v, G(u)≃G(v) -> G(u[t/T])≃G(v[t/T]))
-
-    + reasonable syntactic normalisation
-    + nice rewriting system
-    + confluence without having to deal with connectedness
-    -- reduction for 2p should remain complicated (zig-zags)
-
-
-   B
-    1. 2pdom (for CPP) then 2p
-    2. 2pdom by conservativity
-    3. 2pdom + TaT by simple analysis
-    
-    + target for CPP
-    + 2pdom + TaT not necessary
-    + confluence without having to deal with connectedness (even in the intermediate case with the kill rule)
-    - need 'graphs with a term' for the rewriting system
-    - syntactic normalisation is rather heavy
-
-   C
-    1. 2pdom
-    2. 2p by global analysis
-    3. 2pdom + TaT by simple analysis
-    + simple syntactic normalisation
-    + smaller rewriting system
-    + 2pdom + TaT not necessary
-    - analysis for 2p should be complicated (zig-zags)
-
-   B seems the most reasonable option in the long term ; so for now we focus on B1 for 2pdom
-
-  
-   TOTHINK: algebra of lgraphs v.s. algebra of graphs ???
-   . would be convenient to have some of the laws on lgraphs
-   . current [completeness] theorem, at the end of the file, stated in terms of lgraphs
-     -> need to get 
-     iso (graph_of_term u) (graph_of_term v)  -> liso (lgraph_of_term u) (lgraph_of_term v)
-     (certainly through homomorphism lgraph_of_graph)
- *)
-
-
-(** TOMOVE  *)
-
-Notation "'Σ' x .. y , p" :=
-  (sigT (fun x => .. (sigT (fun y => p%type)) ..))
-  (at level 200, x binder, y binder, right associativity).
-
-Notation IO := [set input; output].
-
-
-Definition S_option A: bij (unit+A) (option A).
-Proof.
-  exists (fun x => match x with inr a => Some a | inl _ => None end)
-         (fun x => match x with Some a => inr a | None => inl tt end);
-    case=>//; case=>//.
-Defined.
-
-Definition two_bool: bij (unit+unit) bool.
-Proof. etransitivity. apply S_option. symmetry. apply bool_option_unit. Defined.
-
-Definition two_option_option_void: bij (unit+unit) (option (option void)).
-Proof.
-  etransitivity. apply bij_sumC.
-  etransitivity. apply S_option.
-  apply option_bij. apply unit_option_void.
-Defined.
-
-Definition merge43: bij (quot (eqv_clot [::(inl true,inr false)])) (option bool).
-Admitted.
-Lemma merge43E:
-  ((merge43 (\pi inl false) = Some false) *
-   (merge43 (\pi inl true) = None) *
-   (merge43 (\pi inr false) = None) *
-   (merge43 (\pi inr true) = Some true))%type.
-Admitted.
-Lemma merge43E':
-  ((merge43^-1 (Some false) = \pi inl false) *
-   (merge43^-1 None = \pi inl true) *
-   (merge43^-1 (Some true) = \pi inr true))%type.
-Admitted.
-
-
-(* TOMOVE *)
-Lemma iso_vbij Lv Le (G: graph Lv Le) (V: finType) (h: bij (vertex G) V):
-  iso G (@Graph _ _ V (edge G)
-                (h \o (@source _ _ G))
-                (h \o (@target _ _ G))
-                ((@vlabel _ _ G) \o h^-1)
-                (@elabel _ _ G)).
-Proof. iso h bij_id. by split=>//= v; rewrite bijK. Defined.
-
-Lemma iso_ebij Lv Le (G: graph Lv Le) (E: finType) (h: bij (edge G) E):
-  iso G (@Graph _ _ (vertex G) E
-                ((@source _ _ G) \o h^-1)
-                ((@target _ _ G) \o h^-1)
-                (@vlabel _ _ G)
-                ((@elabel _ _ G) \o h^-1)).
-Proof. iso bij_id h. by split=>//= v; rewrite bijK. Defined.
-
-Lemma liso_vbij (G: lgraph) (V: finType) (h: bij (vertex G) V):
-  liso G
-       (point (@Graph _ _ V (edge G)
-                      (h \o (@source _ _ G))
-                      (h \o (@target _ _ G))
-                      ((@vlabel _ _ G) \o h^-1)
-                      (@elabel _ _ G))
-              (h input) (h output)).
-Proof. apply (iso_liso (iso_vbij h)). Qed.
-
-Lemma liso_ebij (G: lgraph) (E: finType) (h: bij (edge G) E):
-  liso G
-       (point (@Graph _ _ (vertex G) E
-                ((@source _ _ G) \o h^-1)
-                ((@target _ _ G) \o h^-1)
-                (@vlabel _ _ G)
-                ((@elabel _ _ G) \o h^-1))
-              input output).
-Proof. apply (iso_liso (iso_ebij h)). Qed.
-
-Universe S.
-Inductive step: lgraph -> lgraph -> Type@{S} :=
-  | step_v0: forall G alpha,
-      step
-        (add_vertex G alpha)
-        G
-  | step_v1: forall G x u alpha,
-      step
-        (add_edge (add_vertex G alpha) (Some x) None u)
-        (add_test G x (tst_dom (u·alpha)))
-  | step_v2: forall G x y u alpha v,
-      step
-        (add_edge (add_edge (add_vertex G alpha) (Some x) None u) None (Some y) v)
-        (add_edge G x y (u·alpha·v))
-  | step_e0: forall G x u,
-      step
-        (add_edge G x x u)
-        (add_test G x [1∥u])
-  | step_e2: forall G x y u v,
-      step
-        (add_edge (add_edge G x y u) x y v)
-        (add_edge G x y (u∥v)).
-
-(** It is crucial that we name the universe steps resides in. Without
-the explicit name, the inferred universe is a max-universe, causing
-setoid rewite underneath of steps to fail with the anomaly: "Unable to
-handle arbitrary u+k <= v constraints." *)
-Inductive steps: lgraph -> lgraph -> Type@{S} :=
-  | liso_step: CRelationClasses.subrelation liso steps
-  | cons_step: forall F G H H', liso F G -> step G H -> steps H H' -> steps F H'.
-Existing Instance liso_step.
-
-Instance PreOrder_steps: CRelationClasses.PreOrder steps.
-Proof.
-  split. intro. apply liso_step, liso_id.
-  intros F G H S S'. induction S as [F G I|F G G' G'' I S _ IH].
-  - destruct S' as [F' G' I'|F' G' G'' G''' I' S'].
-    apply liso_step. etransitivity; eassumption.
-    apply cons_step with G' G''=>//. etransitivity; eassumption.
-  - apply cons_step with G G'=>//. by apply IH. 
-Qed.
-
-Instance one_step: CRelationClasses.subrelation step steps.
-Proof. intros F G S. by apply cons_step with F G. Qed.
-
-Definition step_order G H (s: step G H): nat :=
-  match s with
-  | step_v0 _ _ => 0
-  | step_v1 _ _ _ _ => 1
-  | step_v2 _ _ _ _ _ _ => 2
-  | step_e0 _ _ _ => 3
-  | step_e2 _ _ _ _ _ => 4
-  end.
-
-(* Lemmas for manual chaining *)
-Lemma steps_lisoL G G' H : steps G' H -> liso G G' -> steps G H.
-Proof. intros. etransitivity; eauto using liso_step. Qed.
-
-Lemma steps_stepL G G' H : steps G' H -> step G G' -> steps G H.
-Proof. intros. eapply cons_step. reflexivity. eassumption. assumption. Qed.
-
-Lemma steps_comp F G H : steps F G -> steps G H -> steps F H.
-Proof. etransitivity; eassumption. Qed.
-
-
-Instance steps_proper : Proper (liso ==> liso ==> iffT) steps.
-Proof.
-  move => G G' g H H' h. split => S. 
-  - apply: steps_lisoL (liso_sym g). apply: steps_comp S _. exact: liso_step.
-  - apply: steps_lisoL g. apply: steps_comp S _. apply: liso_step. exact: liso_sym.
-Qed. 
-
-Tactic Notation "liso_step" uconstr(h) :=
-  match goal with
-  | |- steps ?G _ => etransitivity;
-                     [apply liso_step;
-                      first [apply h|apply (@liso_vbij G _ h)|apply (@liso_ebij G _ h)]|]
-  | |- liso ?G _ => etransitivity;
-                    [first [apply h|apply (@liso_vbij G _ h)|apply (@liso_ebij G _ h)]|]
-  end.
-
-Proposition local_confluence G G' H H':
-    step G G' -> step H H' -> liso G H -> 
-    {F & steps G' F * steps H' F}%type.
-Admitted.                       (* through open confluence *)
-
-Definition measure (G: lgraph) := #|vertex G| + #|edge G|.
-
-Lemma step_decreases G H: step G H -> measure H < measure G.
-Proof.
-  rewrite /measure.
-  case; intros=>/=; by rewrite !card_option ?addSnnS ?addnS.
-Qed.
-
-Lemma liso_stagnates G H: liso G H -> measure H = measure G.
-Proof. move=>l. by rewrite /measure (card_bij (liso_v l)) (card_bij (liso_e l)). Qed.
-
-Proposition confluence F: forall G H, steps F G -> steps F H -> {F' & steps G F' * steps H F'}%type.
-Proof.
-  induction F as [F_ IH] using (well_founded_induction_type (Wf_nat.well_founded_ltof _ measure)).
-  move=> G H S.
-  move: G H S IH => _ H [F G FG|F__ F0 G' G FF0 FG GG] IH FH.
-  - exists H; split=>//. transitivity F=>//. by apply liso_step, liso_sym.
-  - move: H FH IH FF0=> _ [F H FH|F F1 H' H FF1 FH HH] IH FF0. 
-      exists G; split=>//. transitivity F. by apply liso_step, liso_sym. eauto using cons_step.
-    destruct (local_confluence FG FH) as [M[GM HM]]. transitivity F=>//. by symmetry.
-    destruct (fun D => IH G' D _ _ GG GM) as [L[GL ML]].
-     rewrite /Wf_nat.ltof -(liso_stagnates FF0). apply /ltP. by apply step_decreases.
-    have HL: steps H' L by transitivity M. 
-    destruct (fun D => IH H' D _ _ HL HH) as [R[LR HR]].
-     rewrite /Wf_nat.ltof -(liso_stagnates FF1). apply /ltP. by apply step_decreases.
-     exists R. split=>//. by transitivity L.
-Qed.
-
-
-(** ** 2pdom-operations on graphs *)
-
-Notation merge_seq G l := (@merge _ _ test_monoid G (eqv_clot l)).
-
-(** Note: We choose [unl input] as input and [unr output] as output
-for both binary operations. This allows us to state lemmas for both
-without generalizing only over the sequence *)
-
-Definition lpar (F G: lgraph) :=
-  point (merge_seq (union F G) [::(unl input,unr input); (unl output,unr output)])
-        (\pi (unl input)) (\pi (unr output)).
-
-Definition ldot (F G: lgraph) :=
-  point (merge_seq (union F G) [::(unl output,unr input)])
-        (\pi (unl input)) (\pi (unr output)).
-
-Definition lcnv (F: lgraph) :=
-  point F output input.
-
-Definition ldom (F: lgraph) :=
-  point F input input.
-
-Definition lone :=
-  point (unit_graph [1]) tt tt.
-
-Definition ltop :=
-  point (two_graph [1] [1]) false true.
-
-Definition lvar a :=
-  point (edge_graph [1] (var a) [1]) false true.
-
-Fixpoint lgraph_of_term (u: term): lgraph :=
-  match u with
-  | dot u v => ldot (lgraph_of_term u) (lgraph_of_term v)
-  | par u v => lpar (lgraph_of_term u) (lgraph_of_term v)
-  | cnv u => lcnv (lgraph_of_term u)
-  | dom u => ldom (lgraph_of_term u)
-  | one => lone
-  | var a => lvar a
-  end.
-
-Definition lgraph_of_nf_term (t: nf_term): lgraph :=
-  match t with
-  | nf_test a => point (unit_graph a) tt tt
-  | nf_conn a u b => point (edge_graph a u b) false true
-  end.
-
-(*
-Definition lgraph_of_graph2 (G: graph2): lgraph :=
-  LGraph (@multigraph.source G)
-         (@multigraph.target G)
-         (fun _ => [1])
-         (fun e => var (multigraph.label e))
-         input
-         output.
-
-Lemma lgraph_of_graph2_of_term (u: term): liso (lgraph_of_term u) (lgraph_of_graph2 (graph2_of_term u)).
-Admitted. 
-
-Lemma lgraph_of_graph2_iso (G H: graph2):
-  G ≈ H -> liso (lgraph_of_graph2 G) (lgraph_of_graph2 H).
-Proof.
-  move=>h. exists (iso2_v h) h.e (fun _ => false)=>//; try intro; try apply h.
-    by rewrite /=(label_iso h).
-Qed.
-*)
-
-Lemma dot_liso: Proper (liso ==> liso ==> liso) ldot.
-Proof.
-  move => F F' FF G G' GG. rewrite /ldot.
-  (* setoid_rewrite (iso_liso (merge_iso (union_iso FF GG))). *)
-  (* cannot work: we would need a coercion from liso to iso, which is not true *)
-Admitted.
-
-Lemma par_liso: Proper (liso ==> liso ==> liso) lpar.
-Admitted.
-
-Lemma cnv_liso: Proper (liso ==> liso) lcnv.
-Proof. intros F G l. liso (liso_v l) (liso_e l) (liso_dir l) ; apply l. Qed.
-
-Lemma lcnvC G : liso (lcnv (lcnv G)) G.
-Proof. case: G => G i o. rewrite /lcnv/=. apply: liso_id. Defined.
-
-Lemma dom_liso: Proper (liso ==> liso) ldom.
-Proof. intros F G l. liso (liso_v l) (liso_e l) (liso_dir l); apply l. Qed.
-
-Lemma step_to_steps f:
-  Proper (liso ==> liso) f -> Proper (step ==> steps) f -> Proper (steps ==> steps) f.
-Proof.
-  intros If Sf G G' S.
-  induction S as [G G' I|G G' F H' I S Ss IH].
-  - by apply liso_step, If.
-  - etransitivity. apply liso_step, If, I.
-    etransitivity. apply Sf, S. apply IH. 
-Qed.
-
-Instance cnv_steps: Proper (steps ==> steps) lcnv.
-Proof.
-  apply step_to_steps. by apply cnv_liso.
-  move=>F G S. eapply one_step. destruct S.
-  * apply (@step_v0 (point G output input) alpha).
-  * apply (@step_v1 (point G output input) x u alpha).
-  * apply (@step_v2 (point G output input) x y u alpha v).
-  * apply (@step_e0 (point G output input) x u).
-  * apply (@step_e2 (point G output input) x y u v).
-Qed.
-
-Instance dom_steps: Proper (steps ==> steps) ldom.
-Proof.
-  apply step_to_steps. by apply dom_liso.
-  move=>F G S. eapply one_step. destruct S.
-  * apply (@step_v0 (point G input input) alpha).
-  * apply (@step_v1 (point G input input) x u alpha).
-  * apply (@step_v2 (point G input input) x y u alpha v).
-  * apply (@step_e0 (point G input input) x u).
-  * apply (@step_e2 (point G input input) x y u v).
-Qed.
-
-
-Fixpoint mentions (A  : eqType) (l : pairs A) := flatten [seq [:: x.1;x.2] | x <- l].
-
-Definition admissible_l (G H : lgraph) (e : pairs (union G H)) := 
-  all (fun x => if x is inl z then z \in IO else true) (mentions e).
-
-Definition replace_ioL (G G' H : lgraph) (e : pairs (union G H)) : pairs (union G' H) := 
-  map_pairs (fun (x: union G H) => match x with 
-                   | inl z => if z == output :> G then inl output else inl input
-                   | inr z => inr z
-                   end) e.
-Arguments replace_ioL [G G' H].
-
-Lemma replace_ioE (vT eT1 eT2 :finType) s1 t1 s2 t2 lv1 lv2 le1 le2 i1 i2 o1 o2 H e : admissible_l e -> 
-   i1 = i2 -> o1 = o2 ->                                                                      
-   @replace_ioL (@LGraph (@Graph test_setoid term_setoid vT eT1 s1 t1 lv1 le1) i1 o1) 
-                (@LGraph (@Graph test_setoid term_setoid vT eT2 s2 t2 lv2 le2) i2 o2) H e = e.
-Admitted.
-
-(* Local Notation merge := (@merge test_setoid term_setoid test_monoid). *)
-
-Local Open Scope lgraph_scope.
-
-Lemma iso_merge_add_edgeL (G H : lgraph) x y u e : 
-  iso (merge_seq (union (G ∔ [x,u,y]) H) e) 
-      (multigraph_new.add_edge (merge_seq (union G H) e) (\pi unl x) (\pi unl y) u).
-Admitted.
-
-Definition merge_add_edgeL (G H : lgraph) x y u l i o : 
-  liso (point (merge_seq (union (G ∔ [x,u,y]) H) l) i o)
-       (point (merge_seq (union G H) l) i o ∔ [\pi unl x,u,\pi unl y]).
-Admitted.
-
-Lemma merge_add_edgeLE G H x y u l i o z : @merge_add_edgeL G H x y u l i o z = z.
-Admitted.  
-
-Definition merge_add_testL (G H : lgraph) x a (l : pairs (union (G[tst x <- a]) H)) i o : 
-  liso (point (merge_seq (union (G[tst x <- a]) H) l) i o)
-       ((point (merge_seq (union G H) l) i o)[tst \pi unl x <- a]).
-Admitted.
-
-(*
-Fixpoint pmap_pairs A B (f : A -> option B) (l : pairs A) : pairs B := 
-  match l with 
-  | [::] => [::]
-  | (x,y)::l' => if (f x,f y) is (Some x',Some y') 
-                then (x',y') :: pmap_pairs f l' 
-                else pmap_pairs f l'
-  end.
-
-Fixpoint strip_SomeL A B (l : pairs ((option A) + B)) : pairs (A + B) := 
-  pmap_pairs (fun p => match p with 
-                    | inl (Some x) => Some (inl x)
-                    | inr x => Some (inr x) 
-                    | inl None => None 
-                    end) l.
-*)
-
-Definition merge_add_vertexL (G H : lgraph) a l : admissible_l l ->
-  liso (point (merge_seq (union (G ∔ a) H) l) (\pi (unl input)) (\pi (unr output)))
-       ((point (merge_seq (union G H) (replace_ioL l)) (\pi (unl input)) (\pi (unr output))) ∔ a).
-Admitted.
-
-Lemma merge_add_vertexLE (G H : lgraph) a (l : pairs(union (G ∔ a) H)) (A : admissible_l l) :
-  ((forall x, merge_add_vertexL A (\pi inl (Some x)) = Some (\pi inl x))*
-   (merge_add_vertexL A (\pi inl None) = None))%type.
-Admitted.
-
-Arguments merge_add_edgeL [G H x y u l i o].
-Arguments liso_add_edge [G G'] l [x y u].
-
-Lemma liso_add_edgeE G H l x y u z : @liso_add_edge G H l x y u z = l z. by []. Qed.
-
-Lemma steps_merge (G' G H : lgraph) (l : pairs (union G H)) : 
-  admissible_l l -> step G G' -> 
-  steps (point (merge_seq (union G H) l) (\pi (unl input)) (\pi (unr output)))
-        (point (merge_seq (union G' H) (replace_ioL l)) (\pi (unl input)) (\pi (unr output))).
-Proof.
-  Arguments replace_ioL : clear implicits.
-  move => A B. destruct B. (* why does case fail? *)
-  - admit.
-  - apply: steps_lisoL merge_add_edgeL.
-    apply: steps_lisoL. 2: apply: liso_add_edge. 2: apply (merge_add_vertexL A).
-    rewrite !merge_add_vertexLE.
-    apply: steps_stepL (step_v1 _ _ _ ) .
-    apply: liso_step.  apply: liso_sym. exact: merge_add_testL.
-  - apply: steps_lisoL merge_add_edgeL.
-    apply: steps_lisoL (liso_add_edge (merge_add_edgeL)).
-    rewrite !merge_add_edgeLE. 
-    apply: steps_lisoL (liso_add_edge (liso_add_edge (merge_add_vertexL A))).
-    rewrite [X in steps X _]/=. rewrite !merge_add_vertexLE.
-    apply: steps_stepL (step_v2 _ _ _ _ _) . 
-    exact: steps_lisoL (liso_sym merge_add_edgeL). 
-  - apply: steps_lisoL merge_add_edgeL.
-    apply: steps_stepL (step_e0 _ _).
-    apply: steps_lisoL. 2: apply liso_sym. 2: apply: merge_add_testL.
-    by rewrite replace_ioE.
-  - apply: steps_lisoL merge_add_edgeL.
-    apply: steps_lisoL (liso_add_edge (merge_add_edgeL)).
-    rewrite !merge_add_edgeLE.
-    apply: steps_stepL (step_e2 _ _ _ _).
-    apply: steps_lisoL. 2: apply liso_sym. 2: simpl. 2:exact merge_add_edgeL.
-    by rewrite replace_ioE.
-Admitted.
-
-Lemma step_IO G G' : step G G' -> (input == output :> G) = (input == output :> G').
-Proof. by case. Qed.
-
-Lemma dot_steps_l G G' H: steps G G' -> steps (ldot G H) (ldot G' H).
-Proof.
-  apply (step_to_steps (f:=fun G => ldot G H)) => {G G'}.
-  - apply: (fun _ _ I => dot_liso I liso_id). 
-  - move => G G' stp_G_G'. rewrite /ldot. etransitivity. apply: (@steps_merge G') => //=.
-    + rewrite /admissible_l/=. by rewrite !inE eqxx.
-    + by rewrite /replace_ioL/= eqxx. 
-Qed.
-
-Lemma ldotcnv G H: liso (ldot G H) (lcnv (ldot (lcnv H) (lcnv G))).
-Admitted.
-
-Lemma dot_steps_r G G' H: steps G G' -> steps (ldot H G) (ldot H G').
-Proof.
-  move => GG'. setoid_rewrite ldotcnv.
-  by apply cnv_steps, dot_steps_l, cnv_steps.
-Qed.
-
-Instance dot_steps: Proper (steps ==> steps ==> steps) ldot.
-Proof.
-  repeat intro. by etransitivity; [apply dot_steps_l | apply dot_steps_r].
-Qed.
-
-Lemma lparC G H: liso (lpar G H) (lpar H G).
-Admitted.
-
-Lemma par_steps_l G G' H: steps G G' -> steps (lpar G H) (lpar G' H).
-Proof.
-  apply (step_to_steps (f:=fun G => lpar G H))  => {G G'}. 
-  - move => G G' I. by apply par_liso.
-  - move => G G' step_G_G'. 
-    etransitivity. apply: (@steps_merge G') => //=.
-    + by rewrite /admissible_l/= !inE !eqxx.
-    + rewrite /replace_ioL/= !eqxx. case: ifP => [E|//].
-      rewrite (step_IO step_G_G') in E.
-      by rewrite -[in (inl output,inr input)](eqP E). 
-Qed.
-
-Lemma par_steps_r G G' H: steps G G' -> steps (lpar H G) (lpar H G').
-Proof.
-  intro.
-  etransitivity. apply liso_step, lparC. 
-  etransitivity. 2: apply liso_step, lparC.
-  by apply par_steps_l. 
-Qed.
-
-Instance par_steps: Proper (steps ==> steps ==> steps) lpar.
-Proof.
-  repeat intro. by etransitivity; [apply par_steps_l | apply par_steps_r].
-Qed.
-
-
-Lemma ldotunit G a: liso (ldot G (point (unit_graph a) tt tt)) (add_test G output a).
-Admitted.
-
-Lemma lunitdot G a: liso (ldot (point (unit_graph a) tt tt) G) (add_test G input a).
-Admitted.
-
-Lemma lparunitunit a b:
-  liso (lpar (point (unit_graph a) tt tt) (point (unit_graph b) tt tt))
-       (point (unit_graph [a·b]) tt tt).
-Admitted.
-
-Lemma lparedgeunit a u b c:
-  liso (lpar (point (edge_graph a u b) false true) (point (unit_graph c) tt tt))
-       (point (unit_graph [c∥a·u·b]) tt tt).
-Admitted.
-       
-Lemma add_test_point a c: liso (point (unit_graph a) tt tt [tst tt <- c]) (point (unit_graph [a·c]) tt tt).
-Admitted.                       (* could be inlined for now *)
-
-Lemma add_test_edge (x: bool) a u b c:
-  liso (point (edge_graph a u b) false true [tst x <- c])
-       (point (edge_graph (if x then a else [c·a]) u (if x then [b·c] else b)) false true).
-Admitted.
-
-Proposition reduce (u: term): steps (lgraph_of_term u) (lgraph_of_nf_term (nf u)).
-Proof.
-  induction u=>//=.
-  - etransitivity. apply dot_steps; [apply IHu1|apply IHu2].
-    case (nf u1)=>[a|a u b];
-    case (nf u2)=>[c|c v d]=>/=.
-    * apply liso_step.
-      setoid_rewrite ldotunit. simpl.
-      apply add_test_point. 
-    * apply liso_step.
-      setoid_rewrite lunitdot. simpl.
-      apply add_test_edge. 
-    * apply liso_step.
-      setoid_rewrite ldotunit. simpl.
-      apply add_test_edge. 
-    * rewrite /ldot/=.
-      etransitivity. apply liso_step.
-      2: etransitivity.
-      2: apply one_step, (step_v2 (G:=point (two_graph a d) false true) false true u [b·c] v).
-      2: apply liso_step.
-      2: liso_step (bij_sym unit_option_void)=>/=.
-      2: liso bij_id bij_id (fun _ => false)=>//= _; by rewrite !dotA.
-      liso_step merge43=>/=. 
-      liso_step two_option_option_void=>/=.
-      liso bij_id bij_id (fun _ => false)=>//=;
-           (repeat case)=>//=;
-           rewrite ?merge43E ?merge43E' //=.
-      admit.
-      admit.
-      admit.
-      
-  - etransitivity. apply par_steps; [apply IHu1|apply IHu2].
-    case (nf u1)=>[a|a u b];
-    case (nf u2)=>[c|c v d]=>/=.
-    * apply liso_step. apply lparunitunit.
-    * apply liso_step. setoid_rewrite lparC. apply lparedgeunit.
-    * apply liso_step. apply lparedgeunit.
-    * rewrite /lpar/=.
-      etransitivity. apply liso_step.
-      2: etransitivity.
-      2: apply one_step, (step_e2 (G:=point (two_graph [a·c] [b·d]) false true) false true u v).
-      admit.
-      apply liso_step.
-      liso_step (bij_sym unit_option_void)=>/=. 
-      liso bij_id bij_id (fun _ => false)=>//.
-      
-  - etransitivity. apply cnv_steps, IHu. 
-    case (nf u)=>[a|a v b]=>//=.
-    apply liso_step.
-    rewrite /lcnv/=. liso bool_swap bij_id (fun _ => true)=>//=.
-      by case.
-      move=>_. apply cnvI.
-      
-  - etransitivity. apply dom_steps, IHu. 
-    case (nf u)=>[a|a v b]=>//=.
-    rewrite /ldom/=.
-    etransitivity. apply liso_step.
-    2: etransitivity. 2: apply one_step, (@step_v1 (point (unit_graph a) tt tt) tt v b).
-    simpl.
-    liso_step bool_option_unit=>/=. 
-    liso_step unit_option_void=>/=.
-    liso bij_id bij_id (fun _ => false)=>//=; case=>//.
-    apply liso_step.
-    liso bij_id bij_id (fun _ => false)=>//=; case=>//.
-    apply dotC. 
-Admitted.
-
-Lemma nf_steps s: forall H, steps (lgraph_of_nf_term s) H -> liso (lgraph_of_nf_term s) H.
-Proof.
-  suff E: forall G H, steps G H -> liso G (lgraph_of_nf_term s) -> liso G H
-    by intros; apply E. 
-  destruct 1 as [G H I|G' G H H' I S _ _]=>//L.
-  - exfalso. apply (liso_comp (liso_sym I)) in L. clear -S L. generalize (card_bij (liso_e L)).
-    destruct s; destruct S; simpl in *; (try by rewrite !card_option ?card_unit ?card_void); move=>_.
-    * generalize (card_bij (liso_v L)). rewrite card_unit card_option.
-      have H: 0 < #|G|. apply /card_gt0P. by exists input.
-      revert H. case #|G|; discriminate.
-    * generalize (liso_input L). generalize (liso_output L). simpl.
-      suff E: input=output :>G by congruence.
-      apply (card_le1 (D:=predT))=>//. 
-      apply liso_v, card_bij in L. rewrite card_option card_bool in L.
-        by injection L=>->.
-    * have E: forall y, L None <> L (Some y) by intros y H; generalize (bij_injective (f:=L) H). 
-      case_eq (L None).
-       generalize (liso_output L) (E output). simpl. congruence. 
-       generalize (liso_input L) (E input). simpl. congruence. 
-    * generalize (source_liso L None). generalize (target_liso L None).
-      case liso_dir; simpl; congruence.
-Qed.
-
-Lemma liso_nf (s t: nf_term):
-  liso (lgraph_of_nf_term s) (lgraph_of_nf_term t) ->
-  term_of_nf s ≡ term_of_nf t.
-Proof.
-  case s=>[a|a u b];
-  case t=>[c|c v d]=>/= h.
-  - rewrite -(vlabel_liso h tt). by case (h tt). 
-  - exfalso.
-    generalize (bijK' h false). generalize (bijK' h true).
-    case (h^-1 true). case (h^-1 false). congruence. 
-  - exfalso.
-    generalize (bijK h false). generalize (bijK h true).
-    case (h true). case (h false). congruence.
-  - rewrite -(vlabel_liso h false).
-    rewrite -(vlabel_liso h true).
-    rewrite liso_input liso_output /=. 
-    generalize (elabel_liso h tt).
-    generalize (source_liso h tt).
-    case (liso_dir h tt)=>/=. by rewrite liso_input.
-    by move=>_ ->. 
-Qed.
-
-Theorem completeness (u v: term): liso (lgraph_of_term u) (lgraph_of_term v) -> u ≡ v.
-Proof.
-  move=>h.
-  pose proof (reduce u) as H.
-  have H' : steps (lgraph_of_term u) (lgraph_of_nf_term (nf v))
-    by liso_step h; apply reduce. 
-  case (confluence H H')=>F [/nf_steps HF /nf_steps HF'].
-  rewrite-> (nf_correct u), (nf_correct v).
-  apply liso_nf. liso_step HF. by symmetry. 
-Qed.
+(* 2pdom algebra, initial algebra of terms, tests *)
+
+(* TODO: 2p algebra and their links with 2pdom algebra *)
+
+(* operations are put apart so that the can get notations for them before stating/proving the laws  *)
+Structure ops_ :=
+  { setoid_of_ops:> setoid;
+    dot: setoid_of_ops -> setoid_of_ops -> setoid_of_ops;
+    par: setoid_of_ops -> setoid_of_ops -> setoid_of_ops;
+    cnv: setoid_of_ops -> setoid_of_ops;
+    dom: setoid_of_ops -> setoid_of_ops;
+    one: setoid_of_ops }.
+
+Bind Scope pttdom_ops with setoid_of_ops.
+Delimit Scope pttdom_ops with ptt.
+Open Scope pttdom_ops.
+Notation "x ∥ y" := (par x y) (left associativity, at level 40, format "x ∥ y"): pttdom_ops.
+Notation "x · y" := (dot x y) (left associativity, at level 25, format "x · y"): pttdom_ops.
+Notation "x °"  := (cnv x) (left associativity, at level 5, format "x °"): pttdom_ops.
+Notation "1"  := (one _): pttdom_ops.
+
+Structure pttdom :=
+  { ops:> ops_;
+    dot_eqv: Proper (eqv ==> eqv ==> eqv) (@dot ops);
+    par_eqv: Proper (eqv ==> eqv ==> eqv) (@par ops);
+    cnv_eqv: Proper (eqv ==> eqv) (@cnv ops);
+    dom_eqv: Proper (eqv ==> eqv) (@dom ops);
+    (* domE: forall x: ops, dom x ≡ 1 ∥ x·top; *)
+    parA: forall x y z: ops, x ∥ (y ∥ z) ≡ (x ∥ y) ∥ z;
+    parC: forall x y: ops, x ∥ y ≡ y ∥ x;
+    dotA: forall x y z: ops, x · (y · z) ≡ (x · y) · z;
+    dotx1: forall x: ops, x · 1 ≡ x;
+    cnvI: forall x: ops, x°° ≡ x;
+    cnvpar: forall x y: ops, (x ∥ y)° ≡ x° ∥ y°;
+    cnvdot: forall x y: ops, (x · y)° ≡ y° · x°;
+    par11: 1 ∥ 1 ≡ one ops;
+    A10: forall x y: ops, 1 ∥ x·y ≡ dom (x ∥ y°);
+    (* A11: forall x: ops, x · top ≡ dom x · top; *)
+    (* A12: forall x ops: X, (x∥1) · y ≡ (x∥1)·top ∥ y *)
+    A13: forall x y: ops, dom(x·y) ≡ dom(x·dom y);
+    A14: forall x y z: ops, dom x·(y∥z) ≡ dom x·y ∥ z;
+  }.
+Existing Instances dot_eqv par_eqv cnv_eqv dom_eqv.
+
+Section derived.
+
+ Variable X: pttdom.
+
+ Lemma cnv1: 1° ≡ one X.
+ Proof.
+  rewrite <-dotx1. rewrite <-(cnvI 1) at 2.
+  by rewrite <-cnvdot, dotx1, cnvI.
+ Qed.
+
+ Lemma dot1x (x: X): 1·x ≡ x.
+ Proof. by rewrite <-cnvI, cnvdot, cnv1, dotx1, cnvI. Qed.
+
+ Lemma cnv_inj (x y: X): x° ≡ y° -> x ≡ y.
+ Proof. intro. rewrite <-(cnvI x), <-(cnvI y). by apply cnv_eqv. Qed.
+
+ Lemma dotcnv (x y: X): x·y ≡ (y°·x°)°.
+ Proof. apply cnv_inj. by rewrite cnvdot cnvI. Qed.
+
+ (* dualised equality (to get a bisetoid) *)
+ Definition eqv' (x y: X) := x ≡ y°.
+ Arguments eqv' _ _ /.
+ Lemma eqv'_sym: Symmetric eqv'.
+ Proof. move=> x y /= H. apply cnv_inj. by rewrite cnvI H. Qed.
+ Lemma eqv10 x y z: eqv' x y -> y ≡ z -> eqv' x z.
+ Proof. by move=> /= H <-. Qed.
+ Lemma eqv01 x y z: x ≡ y -> eqv' y z -> eqv' x z.
+ Proof. by move=> /= ->. Qed.
+ Lemma eqv11 x y z: eqv' x y -> eqv' y z -> x ≡ z.
+ Proof. move=> /= -> ->. apply cnvI. Qed.
+ Definition pttdom_bisetoid := BiSetoid eqv'_sym eqv10 eqv01 eqv11. 
+
+ (* tests *)
+ Definition is_test (x: X) := dom x ≡ x.
+ Record test := Test{ elem_of:> X ; testE: is_test elem_of }.
+ Lemma one_test: is_test 1.
+ Admitted.
+ Canonical Structure tst_one := Test one_test. 
+ Lemma dom_test x: is_test (dom x).
+ Admitted.
+ Canonical Structure tst_dom x := Test (dom_test x).
+ Lemma par_test (a: test) (u: X): is_test (a∥u).
+ Admitted.
+ Canonical Structure tst_par a u := Test (par_test a u). 
+ Lemma dot_test (a b: test): is_test (a·b).
+ Admitted.
+ Canonical Structure tst_dot a b := Test (dot_test a b).
+ Lemma cnv_test (a: test): is_test (a°).
+ Admitted.
+ Canonical Structure tst_cnv a := Test (cnv_test a).
+ (* automatised inference of tests *)
+ Definition infer_test x y (e: elem_of y = x) := y.
+ Notation "[ x ]" := (@infer_test x _ erefl).
+
+ (* commutative monoid of  tests *)
+ Definition eqv_test (a b: test) := a ≡ b.
+ Arguments eqv_test _ _ /.
+ Lemma eqv_test_equiv: Equivalence eqv_test.
+ Admitted. 
+ Canonical Structure pttdom_test_setoid := Setoid eqv_test_equiv.
+ Lemma tst_dot_eqv: Proper (eqv ==> eqv ==> eqv) tst_dot.
+ Proof. intros [a] [b] ? [c] [d] ?. by apply dot_eqv. Qed.
+ Lemma tst_dotA: forall a b c: test, [a·[b·c]] ≡ [[a·b]·c].
+ Proof. intros [a] [b] [c]. apply dotA. Qed.
+ Lemma tst_dotC: forall a b: test, [a·b] ≡ [b·a].
+ Admitted.
+ Lemma tst_dotU: forall a: test, [a·1] ≡ a.
+ Proof. intros [a]. apply dotx1. Qed.
+ Canonical Structure pttdom_test_monoid := Monoid tst_dot_eqv tst_dotA tst_dotC tst_dotU.
+ 
+End derived.
+Notation "[ x ]" := (@infer_test _ x _ erefl): pttdom_ops.
+
+
+(* initial algebra of terms *)
+Section terms.
+ Variable A: Type.
+ Inductive term :=
+ | tm_dot: term -> term -> term
+ | tm_par: term -> term -> term
+ | tm_cnv: term -> term
+ | tm_dom: term -> term
+ | tm_one: term
+ | tm_var: A -> term.
+ Bind Scope pttdom_ops with term.
+ Section e.
+ Variable (X: ops_) (f: A -> X).
+ Fixpoint eval (u: term): X :=
+   match u with
+   | tm_dot u v => eval u · eval v
+   | tm_par u v => eval u ∥ eval v
+   | tm_cnv u => (eval u) °
+   | tm_dom u => dom (eval u)
+   | tm_one => 1
+   | tm_var a => f a
+   end.
+ End e.
+ (* axiomatic equality on terms (we do not prove it, but this
+    impredicative encoding is equivalent to the inductive defining
+    equational reasoning in pttdom) *)
+ Definition tm_eqv (u v: term): Prop :=
+   forall (X: pttdom) (f: A -> X), eval f u ≡ eval f v.
+ Hint Unfold tm_eqv.
+ Lemma tm_eqv_equivalence: Equivalence tm_eqv.
+ Proof.
+   constructor.
+     now intro.
+     intros ?? H X f. specialize (H X f). by symmetry. 
+     intros ??? H H' X f. specialize (H X f). specialize (H' X f). etransitivity. apply H. apply H'.
+ Qed.
+ Canonical Structure tm_setoid := Setoid tm_eqv_equivalence. 
+ Canonical Structure tm_ops_ :=
+   {| dot := tm_dot;
+      par := tm_par;
+      cnv := tm_cnv;
+      dom := tm_dom;
+      one := tm_one |}.
+ (* quotiented terms indeed form a pttdom *)
+ Program Definition tm_pttdom: pttdom := {| ops := tm_ops_ |}.
+ Next Obligation. repeat intro; simpl. by apply dot_eqv. Qed.
+ Next Obligation. repeat intro; simpl. by apply par_eqv. Qed.
+ Next Obligation. repeat intro; simpl. by apply cnv_eqv. Qed.
+ Next Obligation. repeat intro; simpl. by apply dom_eqv. Qed.
+ Next Obligation. repeat intro; simpl. by apply parA. Qed.
+ Next Obligation. repeat intro; simpl. by apply parC. Qed.
+ Next Obligation. repeat intro; simpl. by apply dotA. Qed.
+ Next Obligation. repeat intro; simpl. by apply dotx1. Qed.
+ Next Obligation. repeat intro; simpl. by apply cnvI. Qed.
+ Next Obligation. repeat intro; simpl. by apply cnvpar. Qed.
+ Next Obligation. repeat intro; simpl. by apply cnvdot. Qed.
+ Next Obligation. repeat intro; simpl. by apply par11. Qed.
+ Next Obligation. repeat intro; simpl. by apply A10. Qed.
+ Next Obligation. repeat intro; simpl. by apply A13. Qed.
+ Next Obligation. repeat intro; simpl. by apply A14. Qed.
+ Canonical tm_pttdom. 
+ 
+ Notation test := (test tm_pttdom).
+
+ (* TOTHINK: might want to move normalisation to completeness related files *)
+ 
+ (* normal forms for terms *)
+ Inductive nf_term :=
+ | nf_test: test -> nf_term
+ | nf_conn: test -> term -> test -> nf_term.
+
+ Definition term_of_nf (t: nf_term) :=
+   match t with
+   | nf_test alpha => elem_of alpha (* why do we need to insert the coercion??? *)
+   | nf_conn alpha u gamma => alpha · u · gamma
+   end.                                         
+
+ (* pttdom algebra on normal forms *)
+ Definition nf_one := nf_test [1].
+ Definition nf_var a := nf_conn [1] (tm_var a) [1].
+ Definition nf_cnv u :=
+   match u with
+   | nf_test _ => u
+   | nf_conn a u b => nf_conn b (u°) a
+   end.
+ Definition nf_dom u :=
+   match u with
+   | nf_test _ => u
+   | nf_conn a u b => nf_test [a · dom (u·b)]
+   end.
+ Definition nf_dot u v :=
+   match u,v with
+   | nf_test a, nf_test b => nf_test [a·b]
+   | nf_test a, nf_conn b u c => nf_conn [a·b] u c
+   | nf_conn a u b, nf_test c => nf_conn a u [b·c]
+   | nf_conn a u b, nf_conn c v d => nf_conn a (u·b·c·v) d
+   end.
+ Definition nf_par u v :=
+   match u,v with
+   | nf_test a, nf_test b => nf_test [a·b]
+   | nf_test a, nf_conn b u c => nf_test [a ∥ b·u·c]
+   | nf_conn a u b, nf_test c => nf_test [c ∥ a·u·b]
+   | nf_conn a u b, nf_conn c v d => nf_conn [a·c] (u ∥ v) [b·d]
+   end.
+
+ (* normalisation function (could also be defined as an [eval])*)
+ Fixpoint nf (u: term): nf_term :=
+   match u with
+   | tm_dot u v => nf_dot (nf u) (nf v)
+   | tm_par u v => nf_par (nf u) (nf v)
+   | tm_cnv u => nf_cnv (nf u) 
+   | tm_var a => nf_var a
+   | tm_dom u => nf_dom (nf u)
+   | tm_one => nf_one
+   end.
+ 
+ Proposition nf_correct (u: term): u ≡ term_of_nf (nf u).
+ Proof.
+   induction u=>//=.
+   - rewrite {1}IHu1 {1}IHu2.
+     case (nf u1)=>[a|a u b];
+     case (nf u2)=>[c|c v d]=>//=; 
+     rewrite !dotA//.
+   - rewrite {1}IHu1 {1}IHu2.
+     case (nf u1)=>[a|a u b];
+     case (nf u2)=>[c|c v d]=>//=.
+     admit.                      (* ok *)
+     apply parC.
+     admit.                      (* ok *)
+   - rewrite {1}IHu.
+     case (nf u)=>[a|a v b]=>//=.
+     admit.                      (* ok *)
+     rewrite 2!cnvdot dotA.
+     admit. (* ok *)
+   - rewrite {1}IHu.
+     case (nf u)=>[a|a v b]=>//=.
+     admit.                      (* ok *)
+     admit.                      (* ok *)
+   - rewrite dotx1.
+     admit.                      (* ok *)
+ Admitted.
+
+End terms.
