coq/completeness.v
@@ -1,0 +1,116 @@
+Require Import Setoid Morphisms.
+From mathcomp Require Import all_ssreflect.
+Require Import edone preliminaries bij reduction.
+
+Set Implicit Arguments.
+Unset Strict Implicit.
+Unset Printing Implicit Defensive.
+Set Bullet Behavior "Strict Subproofs". 
+
+Section s.
+Variable A: Type.
+Notation test := (test (tm_pttdom A)). 
+Notation term := (term A).
+Notation graph := (graph test term).
+Notation graph2 := (graph2 test term).
+Notation step := (@step A).
+Notation steps := (@steps A).
+
+
+(* /begin 
+ left here for the record, but should disappear since confluence is proved directly via open graphs *)
+Proposition local_confluence G G' H H':
+    step G G' -> step H H' -> G ≃2 H -> 
+    exists F, steps G' F /\ steps H' F.
+Admitted.                       (* through open confluence *)
+Definition measure (G: graph2) := #|vertex G| + #|edge G|.
+Lemma step_decreases G H: step G H -> measure H < measure G.
+Proof.
+  rewrite /measure.
+  case; intros=>/=; by rewrite !card_option ?addSnnS ?addnS.
+Qed.
+Lemma iso_stagnates G H: G ≃2 H -> measure H = measure G.
+Proof. move=>[l _]. by rewrite /measure (card_bij (iso_v l)) (card_bij (iso_e l)). Qed.
+Proposition confluence F: forall G H, steps F G -> steps F H -> exists F', steps G F' /\ steps H F'.
+Proof.
+  induction F as [F_ IH] using (well_founded_induction_type (Wf_nat.well_founded_ltof _ measure)).
+  move=> G H S.
+  move: G H S IH => _ H [F G FG|F__ F0 G' G FF0 FG GG] IH FH.
+  - exists H; split=>//. by rewrite -FG. 
+  - move: H FH IH FF0=> _ [F H FH|F F1 H' H FF1 FH HH] IH FF0. 
+      exists G; split=>//. rewrite -FH. eauto using cons_step.
+    destruct (local_confluence FG FH) as [M[GM HM]]. by rewrite -FF0. 
+    destruct (fun D => IH G' D _ _ GG GM) as [L[GL ML]].
+     rewrite /Wf_nat.ltof -(iso_stagnates FF0). apply /ltP. by apply step_decreases.
+    have HL: steps H' L by transitivity M. 
+    destruct (fun D => IH H' D _ _ HL HH) as [R[LR HR]].
+     rewrite /Wf_nat.ltof -(iso_stagnates FF1). apply /ltP. by apply step_decreases.
+     exists R. split=>//. by transitivity L.
+Qed.
+(* /end  *)
+
+(* graphs of normal forms are in normal form (i.e., can't reduce) *)
+Lemma nf_steps s: forall H, steps (graph_of_nf_term s) H -> graph_of_nf_term s ≃2 H.
+Proof.
+  suff E: forall G H, steps G H -> G ≃2 graph_of_nf_term s -> G ≃2 H.
+    by intros; apply E=>//; reflexivity. 
+  destruct 1 as [G H I|G' G H H' I S _]=>//L.
+  - exfalso. setoid_rewrite I in L. clear -S L. destruct L as [L [Li Lo]]. generalize (card_bij (iso_e L)).
+    destruct s; destruct S; simpl in *; (try by rewrite !card_option ?card_unit ?card_void); move=>_.
+    * generalize (card_bij (iso_v L)). rewrite card_unit card_option.
+      have H: 0 < #|G|. apply /card_gt0P. by exists input.
+      revert H. case #|G|; discriminate.
+    * revert Li Lo. 
+      suff E: input=output :>G by congruence.
+      apply (card_le1 (D:=predT))=>//. 
+      apply iso_v, card_bij in L. rewrite card_option card_bool in L.
+        by injection L=>->.
+    * have E: forall y, L None <> L (Some y) by intros y H; generalize (bij_injective (f:=L) H). 
+      case_eq (L None).
+       generalize (E output). simpl. congruence. 
+       generalize (E input). simpl. congruence. 
+    * generalize (endpoint_iso L false None). generalize (endpoint_iso L true None).
+      case iso_d; simpl; congruence.
+Qed.
+
+(* isomorphisms on graphs of normal forms give back equations *)
+Lemma iso_nf (s t: nf_term A):
+  graph_of_nf_term s ≃2 graph_of_nf_term t ->
+  term_of_nf s ≡ term_of_nf t.
+Proof.
+  case s=>[a|a u b];
+  case t=>[c|c v d]=>/=; move=> [h [hi ho]].
+  - symmetry. exact (vlabel_iso h tt).
+  - exfalso.
+    generalize (bijK' h false). generalize (bijK' h true).
+    case (h^-1 true). case (h^-1 false). congruence. 
+  - exfalso.
+    generalize (bijK h false). generalize (bijK h true).
+    case (h true). case (h false). congruence.
+  - generalize (vlabel_iso h false).
+    generalize (vlabel_iso h true).
+    simpl in *. 
+    rewrite hi ho /=. 
+    generalize (elabel_iso h tt).
+    generalize (endpoint_iso h (h.d tt) tt).
+    case (iso_d h tt)=>/=. by rewrite hi.
+    intros. symmetry. apply dot_eqv=>//. apply dot_eqv=>//. 
+Qed.
+
+(* main completeness theorem *)
+Theorem completeness (u v: term): graph_of_term u ≃2 graph_of_term v -> u ≡ v.
+Proof.
+  move=>h.
+  pose proof (reduce u) as H.
+  have H' : steps (graph_of_term u) (graph_of_nf_term (nf v))
+    by rewrite h; apply reduce. 
+  case (confluence H H')=>F [/nf_steps HF /nf_steps HF'].
+  rewrite-> (nf_correct u), (nf_correct v).
+  apply iso_nf. by rewrite HF'. 
+Qed.
+
+(* TODO: go one step further and get soundness and completeness w.r.t. letter-labelled graphs
+   (using g2_pttdom on the flat bisetoid) *)
+
+End s.
+
