coq/mgraph.v
@@ -1,0 +1,570 @@
+Require Import Setoid Morphisms.
+From mathcomp Require Import all_ssreflect.
+Require Import edone finite_quotient preliminaries bij equiv.
+Require Export pttdom.
+
+Set Implicit Arguments.
+Unset Strict Implicit.
+Unset Printing Implicit Defensive.
+Set Bullet Behavior "Strict Subproofs". 
+
+(* labelled multigraphs and their operations
+   two pointed labelled multigraphs and their operations
+
+TO DO
+ - input/output as a function from [bool]?
+ - ptt algebra on graph2 rather than just pttdom algebra
+
+ *)
+
+Section s.
+  (* note on sectionning
+
+     for now we have three sections in order to assume the least
+     requirements for the various operations/concepts:
+
+     Section s: Lv: Type, Le: Type 
+      (basic defs operations not needing anything) 
+     Section i: Lv: setoid. Le: bisetoid 
+      (notions of homomorphism, isomorphism...)  
+     Section m: Lv: comm_monoid. Le: bisetoid 
+      (operations needing the monoid structure)
+
+     we might want
+     - to put everything in [m] in the end, for the sake of simplicity (in this case, graph2 related things could all be moved to the end) 
+     - to be even more general, e.g., by not assuming setoids for operations like dot/par on graph2, which just need mon0 and mon2
+
+  *)
+    
+Variables Lv Le: Type.
+
+(* labelled multigraphs (not pointed) *)
+Record graph: Type :=
+  Graph {
+      vertex:> finType;
+      edge: finType;
+      endpoint: bool -> edge -> vertex; (* source and target functions *)
+      vlabel: vertex -> Lv;
+      elabel: edge -> Le }.
+Notation source := (endpoint false).
+Notation target := (endpoint true).
+
+(* two pointed graphs (related operations are defined only later) *)
+Record graph2 :=
+  Graph2 {
+      graph_of:> graph;
+      input: vertex graph_of;
+      output: vertex graph_of }.
+Arguments input [_].
+Arguments output [_].
+Notation point G := (@Graph2 G).
+
+
+(* basic graphs and operations *)
+Definition unit_graph a := @Graph [finType of unit] _ (fun _ => vfun) (fun _ => a) vfun.
+Definition two_graph a b := @Graph [finType of bool] _ (fun _ => vfun) (fun v => if v then b else a) vfun.
+Definition edge_graph a u b := Graph (fun b (_: unit) => b) (fun v => if v then b else a) (fun _ => u).                           
+
+Definition add_vertex (G: graph) (l: Lv): graph :=
+  @Graph [finType of option G] (edge G)
+         (fun b e => Some (endpoint b e))
+         (fun v => match v with Some v => vlabel v | None => l end)
+         (@elabel G).
+
+Definition add_vertex2 (G: graph2) (l: Lv): graph2 :=
+  point (add_vertex G l) (Some input) (Some output).
+
+Definition add_edge (G: graph) (x y: G) (l: Le): graph :=
+  @Graph (vertex G) [finType of option (edge G)]
+         (fun b e => match e with Some e => endpoint b e | None => if b then y else x end)
+         (@vlabel G)
+         (fun e => match e with Some e => elabel e | None => l end).
+
+Definition add_edge2 (G: graph2) (x y: G) (u: Le): graph2 :=
+  point (add_edge x y u) input output.
+
+Definition upd_vlabel (G: graph) (x: G) (l: Lv -> Lv): graph :=
+  @Graph (vertex G) (edge G)
+         (@endpoint G)
+         (fun v => if v==x then l (vlabel v) else vlabel v)
+         (@elabel G).
+
+Definition union (G1 G2 : graph) : graph :=
+  {| vertex := [finType of G1 + G2];
+     edge := [finType of edge G1 + edge G2];
+     endpoint b := sumf (@endpoint G1 b) (@endpoint G2 b);
+     vlabel e := match e with inl e => vlabel e | inr e => vlabel e end;
+     elabel e := match e with inl e => elabel e | inr e => elabel e end;
+  |}.
+
+Definition unl {G H: graph} (x: G): union G H := inl x.
+Definition unr {G H: graph} (x: H): union G H := inr x.
+
+End s.
+
+Bind Scope graph_scope with graph.
+Delimit Scope graph_scope with G.
+
+Arguments union {Lv Le} _ _.
+Infix "⊎" := union (at level 50, left associativity) : graph_scope.
+Arguments unl {_ _ _ _}.
+Arguments unr {_ _ _ _}.
+
+Notation "G ∔ [ x , u , y ]" := 
+  (add_edge G x y u) (at level 20, left associativity) : graph_scope.
+Notation "G ∔ a" := 
+  (add_vertex G a) (at level 20, left associativity) : graph_scope.
+
+Bind Scope graph2_scope with graph2.
+Delimit Scope graph2_scope with G2.
+
+Arguments input {_ _ _}.
+Arguments output {_ _ _}.
+Notation point G := (@Graph2 _ _ G).
+
+Notation "G ∔ [ x , u , y ]" := 
+  (@add_edge2 _ _ G x y u) (at level 20, left associativity) : graph2_scope.
+Notation "G ∔ a" := 
+  (add_vertex2 G a) (at level 20, left associativity) : graph2_scope.
+
+Definition merge (Lv: monoid) Le (G : graph Lv Le) (r : equiv_rel G) :=
+  {| vertex := quot r;
+     edge := (edge G);
+     endpoint b e := \pi (endpoint b e);
+     vlabel c := \big[mon2/mon0]_(w | \pi w == c) vlabel w;
+     elabel e := elabel e |}.
+Arguments merge [_ _] _ _.
+Notation merge_seq G l := (merge G (eqv_clot l)).
+
+(* xor operation on Booleans, such that [xor false b] is convertible to [b] *)
+Definition xor b c := if b then negb c else c.
+Lemma xorI a : xor a a = false.
+Proof. by case a. Qed.
+Lemma xorC a b : xor a b = xor b a.
+Proof. by case a; case b. Qed.
+Lemma xorA a b c : xor a (xor b c) = xor (xor a b) c.
+Proof. by case a; case b; case c. Qed.
+
+Section i.
+Variable Lv: setoid.
+Variable Le: bisetoid.
+Notation graph := (graph Lv Le).
+Notation graph2 := (graph2 Lv Le).
+
+(* homomorphisms *)
+Class is_hom (F G: graph) (hv: F -> G) (he: edge F -> edge G) (hd: edge F -> bool): Prop := Hom
+  { endpoint_hom: forall e b, endpoint b (he e) = hv (endpoint (xor (hd e) b) e);
+    vlabel_hom: forall v, vlabel (hv v) ≡ vlabel v;
+    elabel_hom: forall e, elabel (he e) ≡[hd e] elabel e;
+  }.
+(* nota: 
+   - when using the flat_bisetoid for Le, the edge swapping funcion [hd] 
+     may only be constantly false
+   - when the edge swapping function [hd] is constantly false, the
+     types of [endpoint_hom] and [elabel_hom] in the above definition
+     simplify to the simple, non swapping, notion of homomorphism *)
+
+Lemma hom_id G: @is_hom G G id id xpred0.
+Proof. by split. Qed.
+
+Lemma hom_comp F G H hv he hd kv ke kd :
+  @is_hom F G hv he hd -> @is_hom G H kv ke kd -> is_hom (kv \o hv) (ke \o he) (fun e => xor (hd e) (kd (he e))).
+Proof.
+  intros E E'. split.
+  move=>e b=>/=. by rewrite 2!endpoint_hom xorA.
+  move=>x/=. by rewrite 2!vlabel_hom. 
+  move=>e/=.
+  generalize (@elabel_hom _ _ _ _ _ E e). 
+  generalize (@elabel_hom _ _ _ _ _ E' (he e)).
+  case (hd e); case (kd (he e)); simpl.
+  - apply Eqv11. 
+  - apply Eqv01. 
+  - apply Eqv10.
+  - apply transitivity. 
+Qed.
+
+Lemma hom_sym (F G: graph) (hv: bij F G) (he: bij (edge F) (edge G)) hd:
+  is_hom hv he hd -> 
+  is_hom hv^-1 he^-1 (hd \o he^-1).
+Proof.
+  intro H. split.
+  move=>e b=>/=. by rewrite -{3}(bijK' he e) endpoint_hom bijK xorA xorI. 
+  move=>x/=. by rewrite -{2}(bijK' hv x) vlabel_hom.
+  move=>e/=. generalize (@elabel_hom _ _ _ _ _ H (he^-1 e)). rewrite -{3}(bijK' he e) bijK'. apply symmetry. 
+Qed.
+
+(* isomorphisms *)
+
+Record iso (F G: graph): Type :=
+  Iso
+    { iso_v:> bij F G;
+      iso_e: bij (edge F) (edge G);
+      iso_d: edge F -> bool;
+      iso_hom: is_hom iso_v iso_e iso_d }.
+Infix "≃" := iso (at level 79).
+Notation "h '.e'" := (iso_e h) (at level 2, left associativity). 
+Notation "h '.d'" := (iso_d h) (at level 2, left associativity). 
+Global Existing Instance iso_hom.
+
+(* DAMIEN: I did put [iso2] back in Prop (as well as pttdom equality
+   proofs]): I think being in Type is only useful for [iso] (given our
+   application, this would no longer be true if we where to build yet
+   another notion on top of [iso2] where we would need access to the
+   functions) *)
+Definition iso2 (F G: graph2): Prop :=
+  exists f: iso F G, f input = input /\ f output = output. 
+Infix "≃2" := iso2 (at level 79).
+    
+Lemma endpoint_iso F G (h: iso F G) b e: endpoint b (h.e e) = h (endpoint (xor (h.d e) b) e).
+Proof. apply endpoint_hom. Qed.
+
+Lemma vlabel_iso F G (h: iso F G) v: vlabel (h v) ≡ vlabel v.
+Proof. apply vlabel_hom. Qed.
+
+Lemma elabel_iso F G (h: iso F G) e: elabel (h.e e) ≡[h.d e] elabel e.
+Proof. apply elabel_hom. Qed.
+
+Definition iso_id {G}: G ≃ G := @Iso _ _ bij_id bij_id _ (hom_id G). 
+
+Definition iso_sym F G: F ≃ G -> G ≃ F.
+Proof.
+  move => f. 
+  apply Iso with (bij_sym f) (bij_sym f.e) (f.d \o f.e^-1) =>/=.
+  apply hom_sym, f. 
+Defined.
+
+Definition iso_comp F G H: F ≃ G -> G ≃ H -> F ≃ H.
+Proof.
+  move => f g. 
+  eapply Iso with (bij_comp f g) (bij_comp f.e g.e) _=>/=.
+  apply hom_comp. apply f. apply g.
+Defined.
+
+Import CMorphisms.
+
+Global Instance iso_Equivalence: Equivalence iso.
+Proof. constructor. exact @iso_id. exact @iso_sym. exact @iso_comp. Defined.
+
+Global Instance iso2_Equivalence: RelationClasses.Equivalence iso2.
+Proof.
+  split.
+  - intro G. by exists iso_id.
+  - intros F G (f&fi&fo). exists (iso_sym f). by rewrite /= -fi -fo 2!bijK.
+  - intros F G H (f&fi&fo) (g&gi&go). exists (iso_comp f g). 
+    by rewrite /= fi fo gi go.
+Qed.
+
+Lemma endpoint_iso' F G (h: iso F G) b e: endpoint b (h.e^-1 e) = h^-1 (endpoint (xor (h.d (h.e^-1 e)) b) e).
+Proof. apply (endpoint_iso (iso_sym h)). Qed.
+
+Lemma vlabel_iso' F G (h: iso F G) v: vlabel (h^-1 v) ≡ vlabel v.
+Proof. apply (vlabel_iso (iso_sym h)). Qed.
+
+Lemma elabel_iso' F G (h: iso F G) e: elabel (h.e^-1 e) ≡[h.d (h.e^-1 e)] elabel e.
+Proof. apply (elabel_iso (iso_sym h)). Qed.
+
+Definition Iso' (F G: graph)
+           (fv: F -> G) (fv': G -> F)
+           (fe: edge F -> edge G) (fe': edge G -> edge F) fd:
+  cancel fv fv' -> cancel fv' fv ->
+  cancel fe fe' -> cancel fe' fe ->
+  is_hom fv fe fd -> F ≃ G.
+Proof. move=> fv1 fv2 fe1 fe2 E. exists (Bij fv1 fv2) (Bij fe1 fe2) fd. apply E. Defined.
+
+
+(** isomorphisms about union and merge *)
+
+Global Instance union_iso: Proper (iso ==> iso ==> iso) union.
+Proof.
+  intros F F' f G G' g.
+  exists (sum_bij f g) (sum_bij f.e g.e) (fun e => match e with inl e => f.d e | inr e => g.d e end).
+  abstract (split; [
+              move=>[e|e] b/=; by rewrite endpoint_iso |
+              case=>x/=; apply vlabel_iso |
+              case=>e/=; apply elabel_iso ]).
+Defined.
+
+Lemma union_C G H: G ⊎ H ≃ H ⊎ G.
+Proof.
+  exists bij_sumC bij_sumC xpred0.
+  abstract (split; case=>//=). 
+Defined.
+
+Lemma union_A F G H: F ⊎ (G ⊎ H) ≃ F ⊎ G ⊎ H.
+Proof.
+  exists bij_sumA bij_sumA xpred0.
+  abstract by split; case=>[|[|]].
+Defined.
+
+End i.
+Arguments iso {Lv Le}.
+Arguments merge {Lv Le}.
+Infix "≃" := iso (at level 79).
+Notation "h '.e'" := (iso_e h) (at level 2, left associativity). 
+Notation "h '.d'" := (iso_d h) (at level 2, left associativity). 
+Arguments iso2 {Lv Le}.
+Infix "≃2" := iso2 (at level 79).
+
+
+Section m.
+Variable Lv: monoid.
+Variable Le: bisetoid.
+Notation graph := (graph Lv Le).
+Notation graph2 := (graph2 Lv Le).
+
+Section h_merge_nothing'.
+ Variables (F: graph) (r: equiv_rel F).
+ Hypothesis H: forall x y: F, r x y -> x=y.
+ Lemma merge_nothing': merge F r ≃ F.
+ Proof.
+   exists (quot_id H: bij (merge F r) F) bij_id xpred0.
+   split; intros; rewrite /=?quot_idE?H//.
+ Admitted.
+End h_merge_nothing'.
+
+
+Section merge_merge.
+  Variables (F: graph) (e: equiv_rel F) (e': equiv_rel (merge F e)).
+  Lemma hom_merge_merge: is_hom (quot_quot e': merge _ e' -> merge F _) bij_id xpred0.
+  Proof.
+    split; intros=>//. by rewrite /=-equiv_comp_pi.
+  Admitted.
+  Lemma merge_merge: merge (merge F e) e' ≃ merge F (equiv_comp e').
+  Proof. eexists. eapply hom_merge_merge. Defined.
+End merge_merge.
+
+Section merge.
+  Variables (F G: graph) (h: iso F G) (l: pairs F).
+  Definition h_merge: bij (merge_seq F l) (merge_seq G (map_pairs h l)).
+    eapply bij_comp. apply (quot_bij h). apply quot_same. apply eqv_clot_iso.
+  Defined. 
+  Lemma h_mergeE (x: F): h_merge (\pi x) = \pi h x.
+  Proof. by rewrite /=quot_bijE quot_sameE. Qed.
+  Lemma merge_hom: is_hom h_merge h.e h.d.
+  Proof.
+    split; intros=>/=. 
+    - rewrite endpoint_iso. symmetry. apply h_mergeE. 
+    - rewrite quot_sameE. admit. 
+    - apply elabel_iso.
+  Admitted.
+  Definition merge_iso: merge_seq F l ≃ merge_seq G (map_pairs h l) := Iso merge_hom.
+  Lemma merge_isoE (x: F): merge_iso (\pi x) = \pi h x.
+  Proof. apply h_mergeE. Qed.
+End merge.
+Global Opaque h_merge merge_iso.
+
+Section merge_same'.
+ Variables (F: graph) (h k: equiv_rel F).
+ Hypothesis H: h =2 k. 
+ Lemma merge_same'_hom: is_hom (quot_same H: merge _ h -> merge _ k) bij_id xpred0.
+ Proof.
+   split; intros=>//; try (rewrite /=; apply/eqquotP; rewrite -H; apply: piK').
+ Admitted.
+ Definition merge_same': merge F h ≃ merge F k := Iso merge_same'_hom.
+ Lemma merge_same'E (x: F): merge_same' (\pi x) = \pi x.
+ Proof. apply quot_sameE. Qed.
+End merge_same'.
+Global Opaque merge_same'.
+
+Section merge_same.
+ Variables (F: graph) (h k: pairs F).
+ Hypothesis H: eqv_clot h =2 eqv_clot k.
+ Definition merge_same: iso (merge_seq F h) (merge_seq F k) := merge_same' H. 
+ Definition merge_sameE (x: F): merge_same (\pi x) = \pi x := merge_same'E H x. 
+End merge_same.
+Global Opaque merge_same.
+
+
+Section merge_nothing.
+ Variables (F: graph) (h: pairs F).
+ Hypothesis H: List.Forall (fun p => p.1 = p.2) h.
+ Definition merge_nothing: merge_seq F h ≃ F.
+ Proof. apply merge_nothing', eqv_clot_nothing', H. Defined.
+ Lemma merge_nothingE (x: F): merge_nothing (\pi x) = x.
+ Admitted.                      (* need Transparent merge_nothing *)
+ (* Proof. apply quot_idE. Qed. *)
+End merge_nothing.
+Global Opaque merge_nothing.
+
+Section merge_merge_seq.
+  Variables (F: graph) (h k: pairs F) (k': pairs (merge_seq F h)).
+  Hypothesis kk': k' = map_pairs (pi (eqv_clot h)) k.
+  Definition h_merge_merge_seq: bij (merge_seq (merge_seq F h) k') (merge_seq F (h++k)).
+  Proof.
+    eapply bij_comp. apply quot_quot. apply quot_same.
+    rewrite kk'. apply eqv_clot_cat.
+  Defined.
+  Lemma hom_merge_merge_seq: is_hom h_merge_merge_seq bij_id xpred0.
+  Proof.
+    split; intros=>//; try by rewrite /=quot_quotE quot_sameE.
+  Admitted.
+  Definition merge_merge_seq: merge_seq (merge_seq F h) k' ≃ merge_seq F (h++k) :=
+    Iso hom_merge_merge_seq.
+  Lemma merge_merge_seqE (x: F): merge_merge_seq (\pi (\pi x)) = \pi x.
+  Proof. by rewrite /=quot_quotE quot_sameE. Qed.
+End merge_merge_seq.
+Global Opaque merge_merge_seq.
+
+Lemma eqv_clot_map_lr (F G : finType) (l : pairs F) x y : 
+  eqv_clot (map_pairs inl l) (@inl F G x) (@inr F G y) = false.
+Proof. rewrite (@eqv_clot_mapF _) ?inr_codom_inl //. exact: inl_inj. Qed.
+
+Lemma union_equiv_l_eqv_clot (A B: finType) (l: pairs A):
+  union_equiv_l B (eqv_clot l) =2 eqv_clot (map_pairs inl l).
+Proof.
+  rewrite /union_equiv_l/=/union_equiv_l_rel. move => [x|x] [y|y].
+  + rewrite (@eqv_clot_map _ _  _ _ _ (@inl A B)) //. exact: inl_inj.
+  + by rewrite eqv_clot_map_lr.
+  + admit.               (* by rewrite equiv_sym eqv_clot_map_lr.  *) (* STRANGE: was working before *)
+  + by rewrite eqv_clot_map_eq ?sum_eqE // inr_codom_inl.
+Admitted.
+
+Section union_merge_l.
+  Variables (F G: graph) (l: pairs F).
+  Definition h_union_merge_l: bij (merge_seq F l ⊎ G)%G (merge_seq (F ⊎ G) (map_pairs unl l))%G.
+  Proof. eapply bij_comp. apply union_quot_l. apply quot_same. apply union_equiv_l_eqv_clot. Defined.
+  Lemma hom_union_merge_l: is_hom h_union_merge_l bij_id xpred0.
+  Proof.
+    try (split; case; intros=>//=; rewrite ?union_quot_lEl ?union_quot_lEr quot_sameE //).
+  Admitted.
+  Definition union_merge_l: merge_seq F l ⊎ G ≃ merge_seq (F ⊎ G) (map_pairs unl l) :=
+    Iso hom_union_merge_l.
+  Lemma union_merge_lEl (x: F): union_merge_l (inl (\pi x)) = \pi unl x.
+  Proof. by rewrite /=union_quot_lEl quot_sameE. Qed.
+  Lemma union_merge_lEr (x: G): union_merge_l (unr x) = \pi unr x.
+  Proof. by rewrite /=union_quot_lEr quot_sameE. Qed.
+End union_merge_l.  
+Global Opaque union_merge_l.
+
+Lemma map_map_pairs {A B C} (f: A -> B) (g: B -> C) l: map_pairs g (map_pairs f l) = map_pairs (g \o f) l.
+Proof. by rewrite /map_pairs -map_comp. Qed.
+
+Section union_merge_r.
+  Variables (F G: graph) (l: pairs G).
+  Lemma union_merge_r: F ⊎ merge_seq G l ≃ merge_seq (F ⊎ G) (map_pairs unr l).
+  Proof.
+    eapply iso_comp. apply union_C.
+    eapply iso_comp. apply union_merge_l.
+    eapply iso_comp. apply (merge_iso (union_C _ _)).
+    apply merge_same. abstract by rewrite map_map_pairs. 
+  Defined.
+  Lemma union_merge_rEr (x: G): union_merge_r (inr (\pi x)) = \pi (unr x).
+  Proof.
+    (* BUG: the second rewrite hangs if F and x are not given *)
+    rewrite /=. rewrite (union_merge_lEl F _ x).
+    rewrite (merge_isoE (union_C G F) _ (unl x)).
+    by rewrite merge_sameE. 
+  Qed.
+  Lemma union_merge_rEl (x: F): union_merge_r (unl x) = \pi (unl x).
+  Proof.
+    rewrite /=. rewrite (union_merge_lEr _ x) .
+    rewrite (merge_isoE (union_C G F) _ (unr x)).
+    by rewrite merge_sameE. 
+  Qed.
+End union_merge_r.  
+Global Opaque union_merge_r.
+
+Section merge_union_K.
+  Variables (F K: graph) (h: pairs (F+K)) (k: K -> F).
+  Definition union_K_pairs := map_pairs (fun x => match x with inl x => x | inr x => k x end) h.
+
+  Hypothesis kv: forall x: K, vlabel x = mon0.
+  Hypothesis kh: forall x: K, unr x = unl (k x) %[mod (eqv_clot h)].
+
+  Lemma equiv_clot_Kl: union_K_equiv (eqv_clot h) =2 eqv_clot union_K_pairs.
+  Proof.
+    move=> x y. rewrite /union_K_equiv map_equivE. 
+    rewrite !eqv_clotE. set e1 := rel_of_pairs _. set e2 := rel_of_pairs _. 
+    pose j := (fun x => match x with inl x => x | inr x => k x end).
+    apply/idP/idP. 
+    - suff S u v : equiv_of e1 u v -> equiv_of e2 (j u) (j v) by apply: S. 
+      apply: equiv_ofE => {u v} [[u|u] [u'|u']] /= H. 
+      all: rewrite /e2 /j; apply: sub_equiv_of; apply/mapP. 
+      + by exists (unl u,unl u').
+      + by exists (unl u,unr u').
+      + by exists (unr u,unl u').
+      + by exists (unr u,unr u').
+    - apply: equiv_ofE => {x y} x x' xx'. 
+      have kh' z : equiv_of e1 (unr z) (unl (k z)).
+      { rewrite -eqv_clotE. apply/eqquotP. exact: kh. }
+      case/mapP : xx' => [[[u|u] [v|v]] H] /= [-> ->] {x x'}.
+      + exact: sub_equiv_of.
+      + etransitivity. 2: apply kh'. by apply sub_equiv_of. 
+      + etransitivity. symmetry; apply kh'. by apply sub_equiv_of. 
+      + etransitivity. 2: apply kh'. etransitivity. symmetry; apply kh'. by apply sub_equiv_of.
+  Qed.
+  
+  Definition h_merge_union_K: bij (merge_seq (union F K) h) (merge_seq F union_K_pairs).
+    eapply bij_comp. apply quot_union_K with k. apply kh.
+    apply quot_same. apply equiv_clot_Kl. 
+  Defined.
+
+  Hypothesis ke: edge K -> False.
+
+  Definition h_merge_union_Ke1 (e: edge (merge_seq (union F K) h)): edge (merge_seq F union_K_pairs) :=
+    match e with inl e => e | inr e => match ke e with end end.
+
+  Definition h_merge_union_Ke: bij (edge (merge_seq (union F K) h)) (edge (merge_seq F union_K_pairs)).
+    exists h_merge_union_Ke1 inl=>x//. by case x.
+  Defined.
+
+  Lemma hom_merge_union_K: is_hom h_merge_union_K h_merge_union_Ke xpred0.
+  Proof.
+    split; try (case; intros =>//=; by rewrite ?quot_union_KEl ?quot_union_KEr quot_sameE).
+  Admitted.
+
+  Definition merge_union_K: merge_seq (F ⊎ K) h ≃ merge_seq F union_K_pairs :=
+    Iso hom_merge_union_K.
+  Lemma merge_union_KEl (x: F): merge_union_K (\pi (unl x)) = \pi x.
+  Proof. by rewrite /=quot_union_KEl quot_sameE. Qed.
+  Lemma merge_union_KEr (x: K): merge_union_K (\pi (unr x)) = \pi k x.
+  Proof. by rewrite /=quot_union_KEr quot_sameE. Qed.
+End merge_union_K.
+Global Opaque merge_union_K.
+
+
+(* two pointed graphs operations *)
+
+Definition g2_par (F G: graph2) :=
+  point (merge_seq (F ⊎ G) [::(unl input,unr input); (unl output,unr output)])
+        (\pi (unl input)) (\pi (unr output)).
+
+Definition g2_dot (F G: graph2) :=
+  point (merge_seq (F ⊎ G) [::(unl output,unr input)])
+        (\pi (unl input)) (\pi (unr output)).
+
+Definition g2_cnv (F: graph2) :=
+  point F output input.
+
+Definition g2_dom (F: graph2) :=
+  point F input input.
+
+Definition g2_one: graph2 :=
+  point (unit_graph _ mon0) tt tt.
+
+Definition g2_top: graph2 :=
+  point (two_graph _ mon0 mon0) false true.
+
+Definition g2_var a: graph2 :=
+  point (edge_graph mon0 a mon0) false true.
+
+Definition add_test (G: graph2) (x: G) (a: Lv): graph2 :=
+  point (upd_vlabel x (mon2 a)) input output.
+
+(* Note: maybe nicer to prove that this is a ptt algebra (with top)
+  and deduce automatically that this is a pttdom (as we did in the previous version) *)
+Canonical Structure g2_setoid: setoid := Setoid (iso2_Equivalence Lv Le). 
+Canonical Structure g2_ops: ops_ :=
+  {| dot := g2_dot;
+     par := g2_par;
+     cnv := g2_cnv;
+     dom := g2_dom;
+     one := g2_one |}.
+Program Definition g2_pttdom: pttdom := {| ops := g2_ops |}.
+(* TODO: import all isomorphisms... *)
+Admit Obligations.
+Canonical g2_pttdom.
+
+End m. 
+Notation "G [tst x <- a ]" := 
+  (@add_test _ _ G x a) (at level 20, left associativity, format "G [tst  x  <-  a ]") : graph2_scope.
