coq/reduction.v
@@ -1,0 +1,204 @@
+Require Import Setoid Morphisms.
+From mathcomp Require Import all_ssreflect.
+Require Import edone finite_quotient preliminaries bij equiv.
+Require Export rewriting.
+
+Set Implicit Arguments.
+Unset Strict Implicit.
+Unset Printing Implicit Defensive.
+Set Bullet Behavior "Strict Subproofs". 
+
+Section s.
+Variable A: Type.
+Notation test := (test (tm_pttdom A)). 
+Notation term := (term A).
+Notation graph := (graph test term).
+Notation graph2 := (graph2 test term).
+Notation step := (@step A).
+Notation steps := (@steps A).
+
+
+(* algebraic operations preserve rewriting steps *)
+
+Lemma step_to_steps f:
+  Proper (iso2 ==> iso2) f -> Proper (step ==> steps) f -> Proper (steps ==> steps) f.
+Proof.
+  intros If Sf G G' S.
+  induction S as [G G' I|G G' F H' I S Ss IH].
+  - by apply iso_step, If.
+  - etransitivity. apply iso_step, If, I.
+    etransitivity. apply Sf, S. apply IH. 
+Qed.
+
+Instance cnv_steps: Proper (steps ==> steps) (@cnv _).
+Proof.
+  apply step_to_steps. by apply cnv_eqv.
+  move=>F G S. eapply one_step. destruct S.
+  * apply (@step_v0 _ (point G output input) alpha).
+  * apply (@step_v1 _ (point G output input) x u alpha).
+  * apply (@step_v2 _ (point G output input) x y u alpha v).
+  * apply (@step_e0 _ (point G output input) x u).
+  * apply (@step_e2 _ (point G output input) x y u v).
+Qed.
+
+Instance dom_steps: Proper (steps ==> steps) (@dom _).
+Proof.
+  apply step_to_steps. by apply dom_eqv.
+  move=>F G S. eapply one_step. destruct S.
+  * apply (@step_v0 _ (point G input input) alpha).
+  * apply (@step_v1 _ (point G input input) x u alpha).
+  * apply (@step_v2 _ (point G input input) x y u alpha v).
+  * apply (@step_e0 _ (point G input input) x u).
+  * apply (@step_e2 _ (point G input input) x y u v).
+Qed.
+
+Lemma dot_steps_l G G' H: steps G G' -> steps (G·H) (G'·H).
+Proof.
+  apply (step_to_steps (f:=fun G => G·H)) => {G G'}.
+  - move=> ?? E. apply dot_eqv=>//. reflexivity. 
+  - move => G G' GG'. etransitivity. (* apply: (@steps_merge G') => //=. *)
+    (* + rewrite /admissible_l/=. by rewrite !inE eqxx. *)
+    (* + by rewrite /replace_ioL/= eqxx.  *)
+Admitted.
+
+Lemma dot_steps_r G G' H: steps G G' -> steps (H·G) (H·G').
+Proof.
+  move => GG'. rewrite dotcnv. transitivity ((G'°·H°)°). 
+    by apply cnv_steps, dot_steps_l, cnv_steps.
+    by rewrite -dotcnv. 
+Qed.
+
+Instance dot_steps: Proper (steps ==> steps ==> steps) (@dot _).
+Proof.
+  repeat intro. by etransitivity; [apply dot_steps_l | apply dot_steps_r].
+Qed.
+
+Lemma par_steps_l G G' H: steps G G' -> steps (G∥H) (G'∥H).
+Proof.
+  apply (step_to_steps (f:=fun G => (G∥H)))  => {G G'}. 
+  - move => G G' I. apply par_eqv=>//. reflexivity.
+  - move => G G' step_G_G'. 
+    (* etransitivity. apply: (@steps_merge G') => //=. *)
+    (* + by rewrite /admissible_l/= !inE !eqxx. *)
+    (* + rewrite /replace_ioL/= !eqxx. case: ifP => [E|//]. *)
+    (*   rewrite (step_IO step_G_G') in E. *)
+    (*   by rewrite -[in (inl output,inr input)](eqP E).  *)
+Admitted.
+
+Lemma par_steps_r G G' H: steps G G' -> steps (H∥G) (H∥G').
+Proof.
+  intro. rewrite parC. etransitivity. apply par_steps_l. eassumption.
+  by rewrite parC. 
+Qed.
+
+Instance par_steps: Proper (steps ==> steps ==> steps) (@par _).
+Proof.
+  repeat intro. by etransitivity; [apply par_steps_l | apply par_steps_r].
+Qed.
+
+
+(* graphs of terms and normal forms *)
+Definition graph_of_term: term -> graph2 := eval (fun a => g2_var _ (tm_var a)). 
+
+Definition graph_of_nf_term (t: nf_term A): graph2 :=
+  match t with
+  | nf_test a => point (unit_graph _ a) tt tt
+  | nf_conn a u b => point (edge_graph a u b) false true
+  end.
+
+
+(* Some of these isomorphism lemma could be slight generalisations of lemmas
+   used to get the pttdom laws on graph2 *)
+Lemma ldotunit (G: graph2) a: G · point (unit_graph _ a) tt tt ≃2 G [tst output <- a].
+Admitted.
+
+Lemma lunitdot (G: graph2) a: point (unit_graph _ a) tt tt · G ≃2 G [tst input <- a].
+Admitted.
+
+Lemma lparunitunit (a b: test):
+  point (unit_graph term a) tt tt ∥ point (unit_graph _ b) tt tt
+  ≃2 point (unit_graph _ [a·b]) tt tt.
+Admitted.
+
+Lemma lparedgeunit (u: term) (a b c: test):
+  point (edge_graph a u b) false true ∥ point (unit_graph _ c) tt tt
+  ≃2 point (unit_graph _ [c∥a·u·b]) tt tt.
+Admitted.
+       
+Lemma add_test_point (a c: test):
+  point (unit_graph term a) tt tt [tst tt <- c]
+  ≃2 point (unit_graph _ [a·c]) tt tt.
+Admitted.                       (* could be inlined for now *)
+
+Lemma add_test_edge (x: bool) (u: term) (a b c: test):
+  point (edge_graph a u b) false true [tst x <- c]
+  ≃2 point (edge_graph (if x then a else [c·a]) u (if x then [b·c] else b)) false true.
+Admitted.
+
+(* reduction lemma *)
+Proposition reduce (u: term): steps (graph_of_term u) (graph_of_nf_term (nf u)).
+Proof.
+  induction u=>//=.
+  - etransitivity. apply dot_steps; [apply IHu1|apply IHu2].
+    case (nf u1)=>[a|a u b];
+    case (nf u2)=>[c|c v d]=>/=.
+    * apply iso_step.
+      rewrite ldotunit. simpl.
+      apply add_test_point. 
+    * apply iso_step.
+      rewrite lunitdot. simpl.
+      apply add_test_edge. 
+    * apply iso_step.
+      setoid_rewrite ldotunit. simpl.
+      apply add_test_edge. 
+    * etransitivity. apply iso_step.
+      2: etransitivity.
+      2: apply one_step, (step_v2 (G:=point (two_graph _ a d) false true) false true u [b·c] v).
+      2: apply iso_step.
+      (* 2: liso_step (bij_sym unit_option_void)=>/=. *)
+      (* 2: liso bij_id bij_id (fun _ => false)=>//= _; by rewrite !dotA. *)
+      (* liso_step merge43=>/=.  *)
+      (* liso_step two_option_option_void=>/=. *)
+      (* liso bij_id bij_id (fun _ => false)=>//=; *)
+      (*      (repeat case)=>//=; *)
+      (*      rewrite ?merge43E ?merge43E' //=. *)
+      admit.
+      admit.
+      
+  - etransitivity. apply par_steps; [apply IHu1|apply IHu2].
+    case (nf u1)=>[a|a u b];
+    case (nf u2)=>[c|c v d]=>/=.
+    * apply iso_step. apply lparunitunit.
+    * apply iso_step. rewrite parC. apply lparedgeunit.
+    * apply iso_step. apply lparedgeunit.
+    * etransitivity. apply iso_step.
+      2: etransitivity.
+      2: apply one_step, (step_e2 (G:=point (two_graph _ [a·c] [b·d]) false true) false true u v).
+      admit.
+      apply iso_step.
+      (* liso_step (bij_sym unit_option_void)=>/=.  *)
+      (* liso bij_id bij_id (fun _ => false)=>//. *)
+      admit.
+      
+  - etransitivity. apply cnv_steps, IHu. 
+    case (nf u)=>[a|a v b]=>//=.
+    apply iso_step.
+    (* rewrite /lcnv/=. liso bool_swap bij_id (fun _ => true)=>//=. *)
+    (*   by case. *)
+    (*   move=>_. apply cnvI. *)
+    admit.
+      
+  - etransitivity. apply dom_steps, IHu. 
+    case (nf u)=>[a|a v b]=>//=.
+    etransitivity. apply iso_step.
+    2: etransitivity. 2: apply one_step, (@step_v1 _ (point (unit_graph _ a) tt tt) tt v b).
+    (* liso_step bool_option_unit=>/=.  *)
+    (* liso_step unit_option_void=>/=. *)
+    (* liso bij_id bij_id (fun _ => false)=>//=; case=>//. *)
+    (* apply liso_step. *)
+    (* liso bij_id bij_id (fun _ => false)=>//=; case=>//. *)
+    (* apply dotC.  *)
+Admitted.
+
+End s.
+
