coq/structures.v
@@ -1,0 +1,66 @@
+Require Import Setoid Morphisms.
+From mathcomp Require Import all_ssreflect.
+
+Set Implicit Arguments.
+Unset Strict Implicit.
+
+(* basic structures used for the completeness proof of 2pdom algebra
+
+  TODO: packed classes? (does not seem to be problematic for now)
+   but we should at least understand the current hack in rewriting.v for setoid_of_bisetoid
+ *)
+
+
+(* setoids *)
+Structure setoid :=
+  Setoid {
+      car:> Type;
+      eqv: relation car;
+      Eqv: Equivalence eqv
+    }.
+Arguments eqv {_}. 
+Infix "≡" := eqv (at level 79).
+Global Existing Instance Eqv.
+
+(* setoids with an second notion of equality: 
+   - eqv' x y = eqv x y° (when we have an involution _°)
+   - eqv' _ _ = False    (otherwise)
+ *)
+Structure bisetoid :=
+  BiSetoid {
+      setoid_of_bisetoid:> setoid;
+      eqv': relation setoid_of_bisetoid;
+      Eqv'_sym: Symmetric eqv';
+      Eqv10: forall x y z, eqv' x y -> eqv  y z -> eqv' x z;
+      Eqv01: forall x y z, eqv  x y -> eqv' y z -> eqv' x z;
+      Eqv11: forall x y z, eqv' x y -> eqv' y z -> eqv  x z;
+    }.
+Arguments eqv' {_}.
+Infix "≡'" := eqv' (at level 79).
+
+(* switch between [≡] and [≡'] based on a Boolean (useful for defining potentially edge swapping homomorphisms) *)
+Definition eqv_ (X: bisetoid) (b: bool) (x y: X) := if b then x ≡' y else x ≡ y.
+Notation "x ≡[ b ] y" := (eqv_ b x y) (at level 79).
+Global Instance eqv_sym {X: bisetoid} {b}: Symmetric (@eqv_ X b).
+Proof. case b=> x y/=. apply Eqv'_sym. by symmetry. Qed.
+
+Program Definition trivial_bisetoid (X: Type) := {| setoid_of_bisetoid := {| eqv := @eq X |}; eqv' (_ _: X) := False |}.
+Next Obligation. eauto with typeclass_instances. Qed.
+Next Obligation. tauto. Qed.
+
+(* (commutative) monoids 
+   for labelling graph vertices
+ *)
+Structure monoid :=
+  Monoid {
+      setoid_of_monoid:> setoid;
+      mon0: setoid_of_monoid;
+      mon2: setoid_of_monoid -> setoid_of_monoid -> setoid_of_monoid;
+      mon_eqv: Proper (@eqv _ ==> @eqv _ ==> @eqv _) mon2;
+      monA: forall x y z, mon2 x (mon2 y z) ≡ mon2 (mon2 x y) z;
+      monC: forall x y, mon2 x y ≡ mon2 y x;
+      monU: forall x, mon2 x mon0 ≡ x
+    }.
+Global Existing Instance mon_eqv.
+Arguments mon0 {_}.
+Arguments mon2 {_}.
